theories/Printer.v
@@ -1,7 +1,7 @@
 From Coq Require Import String BinInt List.
 
 (* printer for dumping pretty-printed PIR terms to check with the Plutus CLI tool *)
-From SimpleIO Require Import SimpleIO.
+(* From SimpleIO Require Import SimpleIO. *)
 From QuickChick Require Import Show.
 
 From VTL Require Import PIR Pretty Translation.
@@ -9,27 +9,27 @@ From VTL Require Import PIR Pretty Translation.
 Import PlutusNotations ListNotations.
 Local Open Scope string_scope.
 Local Open Scope Z_scope.
-
 Definition identity_ast : term :=
+
   <{ λ "x" :: ℤ, {Var "x"} }>.
 
 Definition plus_ast : term :=
   <{ (λ "x" :: ℤ, λ "y" :: ℤ, {Var "x"} + {Var "y"}) ⋅ CInt 1 }>.
 
-Import IO.Notations.
+(* Import IO.Notations. *)
 
 (* Set stdin/stdout so we can run main from the command line *)
-RunIO IOMode Forward.
+(* RunIO IOMode Forward. *)
 (* Automatically assign the right integer types (hopefully) *)
-RunIO Smart On.
+(* RunIO Smart On. *)
 
 (* We test the pipeline starting from the λ□ identity function *)
 Definition test_pir_ast := (translate_unsafe nil identity_EAst ann_id).
 Eval cbv in (print_as_program test_pir_ast).
-Definition main : IO unit :=
+(* Definition main : IO unit :=
   chan <- open_out "./output/test.pir" ;;
   output_string chan (print_as_program test_pir_ast) ;;
-  close_out chan.
+  close_out chan. *)
 
 (* Getting errors: PrimFloat.float PrimInt63.int have to be realized *)
 (* RunIO main. *)
